Revised Specifications
- Authoritative now uses the binary encoder and decoders.
- Recursive resolver spec completely rewritten and simplified.

src/Examples/DnsServer/AuthoritativeDNSServer.v
@@ -37,7 +37,7 @@ Section BinaryDns.
 
   Variable transformer : Transformer bin.
   Variable transformerUnit : TransformerUnit transformer bool.
-  
+
   Definition encoder x := (x -> CacheEncode -> bin * CacheEncode).
   Definition  decoder x := (bin -> CacheDecode -> x * bin * CacheDecode).
   Variable encode_enum :
@@ -79,7 +79,7 @@ Definition DnsSpec : ADT DnsSig :=
 
     Def Method1 "Process" (this : rep) (b : bin) : rep * bin :=
         p <- {p | fst (encode_packet' p) = b};
-        Repeat recurseDepth initializing n with p!"questions"!"qname"
+        Repeat recurseDepth initializing n with p!"question"!"qname"
                defaulting rec with (ret (buildempty true ``"ServFail" p)) (* Bottoming out w/o an answer signifies a server failure error. *)
         {{ results <- MaxElements (fun r r' : resourceRecord => IsPrefix r!sNAME r'!sNAME)
                              (For (r in this!sRRecords)      (* Bind a list of all the DNS entries *)
@@ -92,14 +92,14 @@ Definition DnsSpec : ADT DnsSig :=
               Then
               b <- SingletonSet (fun b : CNAME_Record =>      (* If the record is a CNAME, *)
                                    List.In (A := resourceRecord) b results
-                                   /\ p!"questions"!"qtype" <> QType_inj CNAME); (* and a non-CNAME was requested*)
+                                   /\ p!"question"!"qtype" <> QType_inj CNAME); (* and a non-CNAME was requested*)
                 Ifopt b as b'
                 Then  (* only one matching CNAME record *)
                   p' <- rec b'!sRDATA; (* Recursively find records matching the CNAME *)
                   ret (add_answer p' b') (* Add the CNAME RR to the answer section *)
                 Else     (* Copy the records with the correct QTYPE into the answer *)
                          (* section of an empty response *)
-                (results <- ⟦ element in results | QType_match (element!sTYPE) (p!"questions"!"qtype") ⟧;
+                (results <- ⟦ element in results | QType_match (element!sTYPE) (p!"question"!"qtype") ⟧;
                   ret (add_answers results (buildempty true ``"NoError" p)))
               Else (* prefix but record's QNAME not an exact match *)
                 (* return all the prefix records that are nameserver records -- *)
@@ -111,6 +111,285 @@ Definition DnsSpec : ADT DnsSig :=
                                  Return rRec;
                  ret (add_additionals glue_results (add_nses (map VariantResourceRecord2RRecord ns_results) (buildempty true ``"NoError" p)))))
           }} >>= fun p => ret (this, fst (encode_packet' p))}.
+
+Theorem DnsManual :
+  FullySharpened DnsSpec.
+Proof.
+Admitted.
+(*start sharpening ADT; unfold DnsSpec.
+  simpl; pose_string_hyps; pose_heading_hyps.
+  hone method "Process".
+  simpl in *.
+  { simplify with monad laws.
+
+    doOne srewrite_each_all drills_each_all finish_each_all.
+    doOne srewrite_each_all drills_each_all finish_each_all.
+    doOne srewrite_each_all drills_each_all finish_each_all.
+    doOne srewrite_each_all drills_each_all finish_each_all.
+    doOne srewrite_each_all drills_each_all finish_each_all.
+    apply refineFueledFix.
+    doOne srewrite_each_all drills_each_all finish_each_all.
+    intros.
+    doOne srewrite_each_all drills_each_all finish_each_all.
+    doOne srewrite_each_all drills_each_all finish_each_all.
+    doOne srewrite_each_all drills_each_all finish_each_all.
+    doOne srewrite_each_all drills_each_all finish_each_all.
+    doOne srewrite_each_all drills_each_all finish_each_all.
+    doOne srewrite_each_all drills_each_all finish_each_all.
+    doOne srewrite_each_all drills_each_all finish_each_all.
+    doOne srewrite_each_all drills_each_all finish_each_all.
+    doOne srewrite_each_all drills_each_all finish_each_all.
+    doOne srewrite_each_all drills_each_all finish_each_all.
+    doOne srewrite_each_all drills_each_all finish_each_all.
+    doOne srewrite_each_all drills_each_all finish_each_all.
+    doOne srewrite_each_all drills_each_all finish_each_all.
+    doOne srewrite_each_all drills_each_all finish_each_all.
+    doOne srewrite_each_all drills_each_all finish_each_all.
+    doOne srewrite_each_all drills_each_all finish_each_all.
+    doOne srewrite_each_all drills_each_all finish_each_all.
+    doOne srewrite_each_all drills_each_all finish_each_all.
+    doOne srewrite_each_all drills_each_all finish_each_all.
+    doOne srewrite_each_all drills_each_all finish_each_all.
+    doOne srewrite_each_all drills_each_all finish_each_all.
+    doOne srewrite_each_all drills_each_all finish_each_all.
+    doOne srewrite_each_all drills_each_all finish_each_all.
+    doOne srewrite_each_all drills_each_all finish_each_all.
+    doOne srewrite_each_all drills_each_all finish_each_all.
+    doOne srewrite_each_all drills_each_all finish_each_all.
+
+    progress doOne srewrite_each_all drills_each_all finish_each_all.
+    doOne srewrite_each_all drills_each_all finish_each_all.
+    doOne srewrite_each_all drills_each_all finish_each_all.
+    doOne srewrite_each_all drills_each_all finish_each_all.
+    doOne srewrite_each_all drills_each_all finish_each_all.
+    doOne srewrite_each_all drills_each_all finish_each_all.
+    doOne srewrite_each_all drills_each_all finish_each_all.
+    doOne srewrite_each_all drills_each_all finish_each_all.
+    doOne srewrite_each_all drills_each_all finish_each_all.
+    doOne srewrite_each_all drills_each_all finish_each_all.
+    doOne srewrite_each_all drills_each_all finish_each_all.
+    doOne srewrite_each_all drills_each_all finish_each_all.
+    doOne srewrite_each_all drills_each_all finish_each_all.
+    doOne srewrite_each_all drills_each_all finish_each_all.
+    doOne srewrite_each_all drills_each_all finish_each_all.
+    doOne srewrite_each_all drills_each_all finish_each_all.
+    doOne srewrite_each_all drills_each_all finish_each_all.
+    doOne srewrite_each_all drills_each_all finish_each_all.
+    doOne srewrite_each_all drills_each_all finish_each_all.
+    doOne srewrite_each_all drills_each_all finish_each_all.
+    doOne srewrite_each_all drills_each_all finish_each_all.
+    doOne srewrite_each_all drills_each_all finish_each_all.
+    doOne srewrite_each_all drills_each_all finish_each_all.
+    doOne srewrite_each_all drills_each_all finish_each_all.
+    doOne srewrite_each_all drills_each_all finish_each_all.
+    doOne srewrite_each_all drills_each_all finish_each_all.
+  }
+  drop_constraintsfrom_DNS.
+  - doAny drop_constraints
+           master_rewrite_drill ltac:(repeat subst_refine_evar; try finish honing).
+  - doOne drop_constraints
+          master_rewrite_drill ltac:(repeat subst_refine_evar; try finish honing).
+    doOne drop_constraints
+          master_rewrite_drill ltac:(repeat subst_refine_evar; try finish honing).
+    doOne drop_constraints
+          master_rewrite_drill ltac:(repeat subst_refine_evar; try finish honing).
+    doOne drop_constraints
+          master_rewrite_drill ltac:(repeat subst_refine_evar; try finish honing).
+doOne drop_constraints
+          master_rewrite_drill ltac:(repeat subst_refine_evar; try finish honing).
+    doOne drop_constraints
+          master_rewrite_drill ltac:(repeat subst_refine_evar; try finish honing).
+    doOne drop_constraints
+          master_rewrite_drill ltac:(repeat subst_refine_evar; try finish honing).
+    doOne drop_constraints
+          master_rewrite_drill ltac:(repeat subst_refine_evar; try finish honing).
+    doOne drop_constraints
+          master_rewrite_drill ltac:(repeat subst_refine_evar; try finish honing).
+    doOne drop_constraints
+          master_rewrite_drill ltac:(repeat subst_refine_evar; try finish honing).
+    doOne drop_constraints
+          master_rewrite_drill ltac:(repeat subst_refine_evar; try finish honing).
+    doOne drop_constraints
+          master_rewrite_drill ltac:(repeat subst_refine_evar; try finish honing).
+    doOne drop_constraints
+          master_rewrite_drill ltac:(repeat subst_refine_evar; try finish honing).
+    doOne drop_constraints
+          master_rewrite_drill ltac:(repeat subst_refine_evar; try finish honing).
+    doOne drop_constraints
+          master_rewrite_drill ltac:(repeat subst_refine_evar; try finish honing).
+    doOne drop_constraints
+          master_rewrite_drill ltac:(repeat subst_refine_evar; try finish honing).
+    doOne drop_constraints
+          master_rewrite_drill ltac:(repeat subst_refine_evar; try finish honing).
+    doOne drop_constraints
+          master_rewrite_drill ltac:(repeat subst_refine_evar; try finish honing).
+    doOne drop_constraints
+          master_rewrite_drill ltac:(repeat subst_refine_evar; try finish honing).
+    doOne drop_constraints
+          master_rewrite_drill ltac:(repeat subst_refine_evar; try finish honing).
+    doOne drop_constraints
+          master_rewrite_drill ltac:(repeat subst_refine_evar; try finish honing).
+    doOne drop_constraints
+          master_rewrite_drill ltac:(repeat subst_refine_evar; try finish honing).
+    doOne drop_constraints
+          master_rewrite_drill ltac:(repeat subst_refine_evar; try finish honing).
+    doOne drop_constraints
+          master_rewrite_drill ltac:(repeat subst_refine_evar; try finish honing).
+    doOne drop_constraints
+          master_rewrite_drill ltac:(repeat subst_refine_evar; try finish honing).
+    doOne drop_constraints
+          master_rewrite_drill ltac:(repeat subst_refine_evar; try finish honing).
+    doOne drop_constraints
+          master_rewrite_drill ltac:(repeat subst_refine_evar; try finish honing).
+    doOne drop_constraints
+          master_rewrite_drill ltac:(repeat subst_refine_evar; try finish honing).
+    doOne drop_constraints
+          master_rewrite_drill ltac:(repeat subst_refine_evar; try finish honing).
+    doOne drop_constraints
+          master_rewrite_drill ltac:(repeat subst_refine_evar; try finish honing).
+    doOne drop_constraints
+          master_rewrite_drill ltac:(repeat subst_refine_evar; try finish honing).
+    doOne drop_constraints
+          master_rewrite_drill ltac:(repeat subst_refine_evar; try finish honing).
+    doOne drop_constraints
+          master_rewrite_drill ltac:(repeat subst_refine_evar; try finish honing).
+    doOne drop_constraints
+          master_rewrite_drill ltac:(repeat subst_refine_evar; try finish honing).
+    doOne drop_constraints
+          master_rewrite_drill ltac:(repeat subst_refine_evar; try finish honing).
+        doOne drop_constraints
+          master_rewrite_drill ltac:(repeat subst_refine_evar; try finish honing).
+  - hone method "AddData".
+    simplify with monad laws; etransitivity; set_evars.
+    doAny simplify_queries
+          Finite_AbsR_rewrite_drill ltac:(repeat subst_refine_evar; try finish honing).
+    doOne srewrite_each_all drills_each_all finish_each_all.
+    doOne srewrite_each_all drills_each_all finish_each_all.
+    doOne srewrite_each_all drills_each_all finish_each_all.
+    doOne srewrite_each_all drills_each_all finish_each_all.
+    setoid_rewrite refine_count_constraint_broken.
+    repeat doOne srewrite_each_all drills_each_all finish_each_all.
+    repeat doOne srewrite_each_all drills_each_all finish_each_all.
+    make_simple_indexes ({|prim_fst := [("FindPrefixIndex", Fin.F1)];
+                           prim_snd := () |} : prim_prod (list (string * Fin.t 6)) ())
+                        ltac:(CombineCase6 BuildEarlyFindPrefixIndex ltac:(LastCombineCase6 BuildEarlyEqualityIndex))
+                               ltac:(CombineCase5 BuildLastFindPrefixIndex ltac:(LastCombineCase5 BuildLastEqualityIndex)).
+    + plan EqIndexUse createEarlyEqualityTerm createLastEqualityTerm
+           EqIndexUse_dep createEarlyEqualityTerm_dep createLastEqualityTerm_dep.
+    + repeat doOne implement_insert''
+            ltac:(master_implement_drill EqIndexUse createEarlyEqualityTerm createLastEqualityTerm; set_evars) ltac:(finish honing).
+    + doOne implement_insert''
+            ltac:(master_implement_drill EqIndexUse createEarlyEqualityTerm createLastEqualityTerm; set_evars) ltac:(finish honing).
+      doOne implement_insert''
+            ltac:(master_implement_drill EqIndexUse createEarlyEqualityTerm createLastEqualityTerm; set_evars) ltac:(finish honing).
+      doOne implement_insert''
+            ltac:(master_implement_drill EqIndexUse createEarlyEqualityTerm createLastEqualityTerm; set_evars) ltac:(finish honing).
+      doOne implement_insert''
+            ltac:(master_implement_drill EqIndexUse createEarlyEqualityTerm createLastEqualityTerm; set_evars) ltac:(finish honing).
+      doOne implement_insert''
+            ltac:(master_implement_drill EqIndexUse createEarlyEqualityTerm createLastEqualityTerm; set_evars) ltac:(finish honing).
+      doOne implement_insert''
+            ltac:(master_implement_drill EqIndexUse createEarlyEqualityTerm createLastEqualityTerm; set_evars) ltac:(finish honing).
+      doOne implement_insert''
+            ltac:(master_implement_drill EqIndexUse createEarlyEqualityTerm createLastEqualityTerm; set_evars) ltac:(finish honing).
+      doOne implement_insert''
+            ltac:(master_implement_drill EqIndexUse createEarlyEqualityTerm createLastEqualityTerm; set_evars) ltac:(finish honing).
+      doOne implement_insert''
+            ltac:(master_implement_drill EqIndexUse createEarlyEqualityTerm createLastEqualityTerm; set_evars) ltac:(finish honing).
+      doOne implement_insert''
+            ltac:(master_implement_drill EqIndexUse createEarlyEqualityTerm createLastEqualityTerm; set_evars) ltac:(finish honing).
+      doOne implement_insert''
+            ltac:(master_implement_drill EqIndexUse createEarlyEqualityTerm createLastEqualityTerm; set_evars) ltac:(finish honing).
+      doOne implement_insert''
+            ltac:(master_implement_drill EqIndexUse createEarlyEqualityTerm createLastEqualityTerm; set_evars) ltac:(finish honing).
+      doOne implement_insert''
+            ltac:(master_implement_drill EqIndexUse createEarlyEqualityTerm createLastEqualityTerm; set_evars) ltac:(finish honing).
+      doOne implement_insert''
+            ltac:(master_implement_drill EqIndexUse createEarlyEqualityTerm createLastEqualityTerm; set_evars) ltac:(finish honing).
+      doOne implement_insert''
+            ltac:(master_implement_drill EqIndexUse createEarlyEqualityTerm createLastEqualityTerm; set_evars) ltac:(finish honing).
+      doOne implement_insert''
+            ltac:(master_implement_drill EqIndexUse createEarlyEqualityTerm createLastEqualityTerm; set_evars) ltac:(finish honing).
+      doOne implement_insert''
+            ltac:(master_implement_drill EqIndexUse createEarlyEqualityTerm createLastEqualityTerm; set_evars) ltac:(finish honing).
+doOne implement_insert''
+            ltac:(master_implement_drill EqIndexUse createEarlyEqualityTerm createLastEqualityTerm; set_evars) ltac:(finish honing).
+      doOne implement_insert''
+            ltac:(master_implement_drill EqIndexUse createEarlyEqualityTerm createLastEqualityTerm; set_evars) ltac:(finish honing).
+
+
+      doOne implement_insert''
+            ltac:(master_implement_drill EqIndexUse createEarlyEqualityTerm createLastEqualityTerm; set_evars) ltac:(finish honing).
+      doOne implement_insert''
+            ltac:(master_implement_drill EqIndexUse createEarlyEqualityTerm createLastEqualityTerm; set_evars) ltac:(finish honing).
+      doOne implement_insert''
+            ltac:(master_implement_drill EqIndexUse createEarlyEqualityTerm createLastEqualityTerm; set_evars) ltac:(finish honing).
+      doOne implement_insert''
+            ltac:(master_implement_drill EqIndexUse createEarlyEqualityTerm createLastEqualityTerm; set_evars) ltac:(finish honing).
+      doOne implement_insert''
+            ltac:(master_implement_drill EqIndexUse createEarlyEqualityTerm createLastEqualityTerm; set_evars) ltac:(finish honing).
+      doOne implement_insert''
+            ltac:(master_implement_drill EqIndexUse createEarlyEqualityTerm createLastEqualityTerm; set_evars) ltac:(finish honing).
+      doOne implement_insert''
+            ltac:(master_implement_drill EqIndexUse createEarlyEqualityTerm createLastEqualityTerm; set_evars) ltac:(finish honing).
+      doOne implement_insert''
+            ltac:(master_implement_drill EqIndexUse createEarlyEqualityTerm createLastEqualityTerm; set_evars) ltac:(finish honing).
+      doOne implement_insert''
+            ltac:(master_implement_drill EqIndexUse createEarlyEqualityTerm createLastEqualityTerm; set_evars) ltac:(finish honing).
+      doOne implement_insert''
+            ltac:(master_implement_drill EqIndexUse createEarlyEqualityTerm createLastEqualityTerm; set_evars) ltac:(finish honing).
+      doOne implement_insert''
+            ltac:(master_implement_drill EqIndexUse createEarlyEqualityTerm createLastEqualityTerm; set_evars) ltac:(finish honing).
+      doOne implement_insert''
+            ltac:(master_implement_drill EqIndexUse createEarlyEqualityTerm createLastEqualityTerm; set_evars) ltac:(finish honing).
+      doOne implement_insert''
+            ltac:(master_implement_drill EqIndexUse createEarlyEqualityTerm createLastEqualityTerm; set_evars) ltac:(finish honing).
+      doOne implement_insert''
+            ltac:(master_implement_drill EqIndexUse createEarlyEqualityTerm createLastEqualityTerm; set_evars) ltac:(finish honing).
+      doOne implement_insert''
+            ltac:(master_implement_drill EqIndexUse createEarlyEqualityTerm createLastEqualityTerm; set_evars) ltac:(finish honing).
+      doOne implement_insert''
+            ltac:(master_implement_drill EqIndexUse createEarlyEqualityTerm createLastEqualityTerm; set_evars) ltac:(finish honing).
+      Focused_refine_TopMost_Query.
+      implement_In_opt.
+      repeat progress distribute_filters_to_joins.
+      implement_filters_with_find
+        ltac:(find_simple_search_term ltac:(CombineCase5 PrefixIndexUse EqIndexUse)
+                      ltac:(CombineCase10 createEarlyPrefixTerm createEarlyEqualityTerm)
+                             ltac:(CombineCase7 createLastPrefixTerm createLastEqualityTerm))
+               ltac:(find_simple_search_term_dep
+                       ltac:(CombineCase7 PrefixIndexUse_dep EqIndexUse_dep)
+                              ltac:(CombineCase11 createEarlyPrefixTerm_dep createEarlyEqualityTerm_dep)
+                                     ltac:(CombineCase8 createLastPrefixTerm_dep createLastEqualityTerm_dep)).
+
+
+
+      doOne implement_insert''
+            ltac:(master_implement_drill EqIndexUse createEarlyEqualityTerm createLastEqualityTerm; set_evars) ltac:(finish honing).
+      implement_In_opt.
+      repeat progress distribute_filters_to_joins.
+      setoid_rewrite
+      match goal with
+  | [H : @DelegateToBag_AbsR ?qs_schema ?indexes ?r_o ?r_n
+     |- refine (UnConstrQuery_In (ResultT := ?resultT) ?r_o ?idx ?f) _ ] =>
+    etransitivity;
+      [ let H' := eval simpl in (refine_Filtered_Query_In_Enumerate H (idx := idx) f) in
+            apply H'
+      | apply refine_under_bind; intros; implement_In_opt' ]
+
+  | [H : @DelegateToBag_AbsR ?qs_schema ?indexes ?r_o ?r_n
+     |- refine (List_Query_In ?b (fun b : ?QueryT => Where (@?P b) (@?resultComp b))) _ ] =>
+    etransitivity;
+      [ let H' := eval simpl in (@refine_List_Query_In_Where QueryT _ b P resultComp _) in
+            apply H'
+      | implement_In_opt'; implement_In_opt' ] end.
+
+
+    +  unfold SearchUpdateTerm in Index; simpl in Index.
+       simpl.
+Finish_Master ltac:(CombineCase6 BuildEarlyTrieBag  BuildEarlyBag )
+                           ltac:(CombineCase5 BuildLastTrieBag BuildLastBag).
+Time Defined. *)
 
 End BinaryDns.
 
@@ -136,7 +415,7 @@ Definition DnsSpec (recurseDepth : nat) : ADT DnsSig :=
       Insert t into this!sRRecords,
 
     Def Method1 "Process" (this : rep) (p : packet) : rep * packet :=
-        Repeat recurseDepth initializing n with p!"questions"!"qname"
+        Repeat recurseDepth initializing n with p!"question"!"qname"
                defaulting rec with (ret (buildempty true ``"ServFail" p)) (* Bottoming out w/o an answer signifies a server failure error. *)
         {{ results <- MaxElements (fun r r' : resourceRecord => IsPrefix r!sNAME r'!sNAME)
                              (For (r in this!sRRecords)      (* Bind a list of all the DNS entries *)
@@ -149,14 +428,14 @@ Definition DnsSpec (recurseDepth : nat) : ADT DnsSig :=
               Then
               b <- SingletonSet (fun b : CNAME_Record =>      (* If the record is a CNAME, *)
                                    List.In (A := resourceRecord) b results
-                                   /\ p!"questions"!"qtype" <> QType_inj CNAME); (* and a non-CNAME was requested*)
+                                   /\ p!"question"!"qtype" <> QType_inj CNAME); (* and a non-CNAME was requested*)
                 Ifopt b as b'
                 Then  (* only one matching CNAME record *)
                   p' <- rec b'!sRDATA; (* Recursively find records matching the CNAME *)
                   ret (add_answer p' b') (* Add the CNAME RR to the answer section *)
                 Else     (* Copy the records with the correct QTYPE into the answer *)
                          (* section of an empty response *)
-                (results <- ⟦ element in results | QType_match (element!sTYPE) (p!"questions"!"qtype") ⟧;
+                (results <- ⟦ element in results | QType_match (element!sTYPE) (p!"question"!"qtype") ⟧;
                   ret (add_answers results (buildempty true ``"NoError" p)))
               Else (* prefix but record's QNAME not an exact match *)
                 (* return all the prefix records that are nameserver records -- *)
