src/Examples/DnsServer/RecursiveDNSSchema.v
@@ -77,9 +77,6 @@ Definition sSLIST_ORDERS := "SLIST orders".
 Definition sTIME_LAST_CALCULATED := "Time the TTL was last calculated".
 Local Open Scope Heading_scope.
 
-(* Unique Request IDs *)
-Definition ID : Type := word 16.
-
 (* Heading for a pending request. This is a packet plus a *)
 (* unique ID associated with the request and a timeout for *)
 (* discarding stale requests. *)
@@ -98,7 +95,7 @@ Definition RequestHeading : Heading :=
 (* list. *)
 Definition SLISTHeading :=
   < sQUERYCOUNT :: W, (* number of times we've queried this server *)
-    sTTL :: timeT, (* Domain of known server *)
+    sTTL :: timeT, (* remaining time to live of known server *)
     sDOMAIN :: DomainName, (* Domain of known server *)
     sIP :: W > (* Address of server. *).
 
@@ -111,15 +108,18 @@ Definition CacheType :=
 (* according to RFC 2308. The SOA's TTL is used as the length of *)
 (* time to assume a name failure. *)
 
+Definition FailureRecord :=
+  @Tuple (<"RCODE" :: ResponseCode> ++ SOAHeading).
+
 Definition CachedValueTypes :=
-  [ resourceRecord; SOA_Record ].
+  [ resourceRecord; FailureRecord ].
 
 Definition CachedValue := SumType CachedValueTypes.
 
 Definition rRecord2CachedValue (vrr : resourceRecord)
   : CachedValue := inj_SumType CachedValueTypes (ibound (indexb (Bound := ["Answer"; "Failure"]) ``"Answer")) vrr.
 
-Definition Failure2CachedValue (vrr : SOA_Record)
+Definition Failure2CachedValue (vrr : FailureRecord)
   : CachedValue := inj_SumType CachedValueTypes (ibound (indexb (Bound := ["Answer"; "Failure"]) ``"Failure")) vrr.
 
 (* Only cache specific resource records in response to a query. *)
@@ -131,7 +131,7 @@ Definition CachedQueryTypes_inj (rr : CachedQueryTypes) : QType :=
 
 Coercion CachedQueryTypes_inj : CachedQueryTypes >-> QType.
 Coercion rRecord2CachedValue : resourceRecord >-> CachedValue.
-Coercion Failure2CachedValue : SOA_Record >-> CachedValue.
+Coercion Failure2CachedValue : FailureRecord >-> CachedValue.
 
 Definition CacheHeading :=
   < sTTL :: timeT, (* Lifetime of cached value *)
@@ -149,331 +149,9 @@ Definition RecResolverSchema :=
           relation sCACHE has schema CacheHeading ]
         enforcing [ ].
 
-Definition requestTTL : timeT := natToWord _ 0.
-
 (* Should probably restrict cache to have either an answer *)
 (* or a failure for a domain and question type. *)
 
-Open Scope Tuple_scope.
-
-Definition DnsSpec : ADT _ :=
-  Def ADT {
-    rep := QueryStructure RecResolverSchema,
-
-    Def Constructor "Init" : rep := empty,,
-
-    Def Method3 "Process"
-        (this : rep)
-        (sourceIP : W)
-        (curTime : timeT)
-        (p : packet) : rep * packet * W :=
-      If p!"QR" Then
-         (* It's a new request! *)
-         vs <- For (v in this!sCACHE) (* Search cache for an answer *)
-              Where (p!"questions"!"qtype" = CachedQueryTypes_inj v!sQTYPE)
-              Where (curTime <= v!sTTL) (* only alive cached values *)
-              Return (v ! sCACHEDVALUE) ;
-         If is_empty vs Then (* Need to launch a recursive query *)
-                  (* Step 1: Generate a unique ID for the new request. *)
-            (reqIDs <- For (req in this!sREQUESTS)
-                       Where (curTime <= req!sTTL)
-                       Return (req!sID);
-             newID <- { newID | ~ List.In newID reqIDs};
-             (* Find the best known servers to query *)
-             bestServer <- MaxElement
-                             (fun r r' : @Tuple SLISTHeading =>
-                                IsPrefix r!sDOMAIN r'!sDOMAIN
-                                /\ r!sQUERYCOUNT <= r'!sQUERYCOUNT)
-                             (For (server in this!sSLIST)
-                              Where (IsPrefix server!sDOMAIN p!"questions"!"qname")
-                              Where (curTime <= server!sTTL)
-                              Return server);
-             Ifopt bestServer as bestServer Then (* Pick the first server*)
-             `(this, b) <- Insert < sID :: newID,
-                                    sIP :: sourceIP,
-                                    sTTL :: requestTTL > ++ p into this!sREQUESTS;
-             ret (this, (<"id" :: newID,
-                             "QR" :: false,
-                             "Opcode" :: ``"Query",
-                             "AA" :: false,
-                             "TC" :: false,
-                             "RD" :: true,
-                             "RA" :: false,
-                             "RCode" :: ``"NoError",
-                             "question" :: p!"questions",
-                             "answers" :: [ ],
-                             "authority" :: [ ],
-                             "additional" :: [ ] >, bestServer!sIP))
-             Else (* There are no known servers that can answer this request. *)
-             ret (this, (buildempty false ``"ServFail" p, sourceIP)) (* This won't happen if the server has been properly initialized with the root servers. *)
-            )
-       Else                   (* Return cached answer *)
-         (answers <- { answers | forall ans : resourceRecord, List.In ans answers <-> List.In (A := CachedValue) ans vs };
-          If is_empty answers Then (* It must be a cached failure *)
-             failures <- { failures | forall fail : SOA_Record, List.In (A := resourceRecord) fail failures <-> List.In (A := CachedValue) fail vs };
-             ret (this, (add_additionals failures (buildempty false ``"NXDomain" p), sourceIP)) (* Add the SoA record to additional and return negative result*)
-          Else
-          ret (this, (add_answers answers (buildempty false ``"NoError" p), sourceIP)))
-         (* Add the answers to the packet.  *)
-      Else (* It's a response, so we need to associate the packet with *)
-           (* an in-flight request. *)
-      ret (this, (p, natToWord _ 0))
-        }.
-
-
-(* TODO the SOA is technically supposed to go in the Authority section
-but the packet type doesn't include it *)
-
-
-
-(* position in SLIST *)
-Definition position := W.
-(* e.g. ["192", "168", "1", "1"] *)
-Definition IP := DomainName.
-
-(* Type of the things that we (the server) can send to the wrapper, including *)
-(* various error codes and responses. *)
-Inductive ToOutside : Type :=
-(* Errors *)
-| InvalidQuestion : id -> ToOutside
-| InvalidResponse : id -> ToOutside
-| InvalidPacket : id -> packet -> ToOutside
-| MissingSOA : id -> packet -> ToOutside
-| InternalCacheError : id -> packet -> ToOutside
-| NoReferralsLeft : id -> packet -> ToOutside
-| InvalidId : id -> packet -> ToOutside
-(* Responses *)
-(* We were referred to the server with ip IP, and ask it the same question. *)
-(* Request is pending *)
-| ServerQuestion : id -> IP -> packet -> ToOutside
-(* Request is finished *)
-| ClientAnswer : id -> packet -> ToOutside
-| ClientFailure : id -> packet -> SOA_RDATA -> ToOutside.
-
-(* Type of things we store for a finished request. (Note no referrals) *)
-Inductive ToStore : Type :=
-| Answer : DomainName -> packet -> ToStore
-| Failure : DomainName -> packet -> SOA_RDATA -> ToStore.
-
-(* The section of a packet that a certain answer (DNSRRecord) is in, *)
-(* used to tag the flattened rows from a packet. Needed because they're *)
-(* all of type answer so there's no other way to distinguish them *)
-Inductive PacketSection : Type :=
-| PAnswer : PacketSection
-| PAuthority : PacketSection
-| PAdditional : PacketSection.
-
-
-(* ------------------ Schema headings *)
-
-(* The ideal schema would be domain and WrapperResponse, with some way *)
-(* to query the types nested in WrapperResponse. Flattening it here has *)
-(* the same effect. *)
-
-(* One (Domain => WrapperResponse) mapping is flattened into several rows *)
-(* that all have the same packet information, but store one answer *)
-(* (DNSRRecord) each. *)
-
-(* When removing a (Domain => ToStore): delete rows with the Domain in *)
-(* all cache tables. *)
-
-(* When inserting/updating a new (Domain => ToStore): after checking that *)
-(* Domain doesn't exist in any of the cache tables (or just performing a *)
-(* delete), flatten it and insert each row. *)
-
-(* Invariants: (TODO) *)
-(* - All rows for each domain should appear in exactly 1 of the cache *)
-(*   relations (question, answer, or failure). We do not store multiple *)
-(*   possibilities. *)
-(* - All rows for each domain should have the same packet info. *)
-
-(* Heading for cached referrals. Same as above but without the "live" *)
-(* information (ids, match and query count) and with cache info (TTL and *)
-(* time the TTL was last calculated) *)
-
-Definition ReferralHeading :=
-  (* R- = referral domain's, S- = server domain's *)
-  < sREFERRALDOMAIN :: DomainName,
-    sRTYPE :: RRecordType,
-    sRCLASS :: RRecordClass,
-    sRTTL :: W,
-    (* inline RDATA and additional record *)
-    sSERVERDOMAIN :: DomainName,
-    sSTYPE :: RRecordType,
-    sSCLASS :: RRecordClass,
-    sSTTL :: W,
-    sSIP :: DomainName,
-    (* IP in RDATA of additional record *)
-    sTIME_LAST_CALCULATED :: timeT
->.
-
-(*  Stores a cached answer (DNSRRecord). Might have appeared in the *)
-(*  answer, authority, or additional section of a packet. *)
-(*  sDOMAIN and sNAME may differ in the case of CNAME, where *)
-(*  sDOMAIN is an alias for sNAME. See RFC 1034, 6.2.7  *)
-
-Definition AnswerHeading :=
-  < sDOMAIN :: DomainName,
-    sPACKET_SECTION :: PacketSection,
-    sTIME_LAST_CALCULATED :: timeT>
-    ++ resourceRecordHeading.
-
-(* Stores an SOA (Start of Authority) record for cached failures,
-according to RFC 2308. The SOA's TTL is used as the length of time to
-assume a name failure *)
-
-(* TODO the SOA is technically supposed to go in the Authority section
-but the packet type doesn't include it *)
-
-Definition FailureHeading :=
-  < sDOMAIN :: DomainName,
-    sTIME_LAST_CALCULATED :: timeT>
-    ++ SOAHeading.
-
-Definition ReferralRow := @Tuple ReferralHeading.
-Definition SLIST_ReferralRow := @Tuple SLIST_ReferralHeading.
-Definition AnswerRow := @Tuple AnswerHeading.
-Definition FailureRow := @Tuple FailureHeading.
-Definition RequestRow := @Tuple RequestHeading.
-
-(* Type of things that a cache query can return.
-Process gets ALL the rows that match; we don't do any filtering.
-Process deals with re-hierarchizing, choosing the best result, etc. *)
-Inductive CacheResult :=
-| Nope : CacheResult
-(* Nonempty lists *)
-| Ref : list ReferralRow -> CacheResult
-| Ans : list AnswerRow -> CacheResult
-(* A failure stores exactly one result (the SOA) *)
-| Fail : option FailureRow -> CacheResult.
-
-(* Type used in the cache pointer table, which maps names that exist in the cache
-somewhere to the table that they're in.
-We need to cache referrals, but never in relation to a specific name, which is why
-they're not in this type. (For a particular request with a name, it will always end in Answer or Failure) *)
-Inductive CacheTable :=
-| CAnswers
-| CFailures.
-
-(* Type for SLIST order. See RFC 1034, page 32 for a more detailed
-description of the SLIST.
-
-SLIST: a structure which describes the name servers and the
-       zone which the resolver is currently trying to query.
-       This structure keeps track of the resolver's current
-       best guess about which name servers hold the desired
-       information; it is updated when arriving information
-       changes the guess.
-
-Here, an SLIST is a list of current referrals we have, sorted by
-descending match count (so the first one to be used should have the
-highest match count). (TODO: should also incorporate query count) We
-store the referrals in one table and their positions in another
-table. Each request's SLIST is a list of (refId, position).
-
-The SLIST is deleted after a request finishes (ends in an answer or
-failure). Individual referrals may be cleared when their TTL runs
-out. *)
-Record refPosition := { refId : id; refPos : W }.
-
-Definition DnsRecSchema :=
-  Query Structure Schema
-        [ relation sREQUESTS has
-                   schema
-                   RequestHeading;
-
-            (* (* Described above *) *)
-            (* (* caching optimization opportunity!!!! (ACTION ITEM) *) *)
-            (* relation sSLIST_ORDERS has schema *)
-            (*          < sREQID :: id, *)
-            (*            sORDER :: list refPosition *)
-            (*                   (* id instead + func *) *)
-            (*          >; *)
-            (*          (* reqid, refid, refpos *) *)
-            relation sSLIST has
-                     schema
-                     SLIST_ReferralHeading;
-
-            relation sCACHE_POINTERS has schema
-            < sDOMAIN :: DomainName,
-            sCACHETABLE :: CacheTable
-            (* would like to have a variant type in the schema *)
-            > ;
-            relation sCACHE_ANSWERS has
-                     schema
-                     AnswerHeading;
-            relation sCACHE_REFERRALS has
-                     schema
-                     ReferralHeading;
-            relation sCACHE_FAILURES has
-                     schema
-                     FailureHeading
-        ]
-        enforcing [ ].
-(* where (fun t t' => True) ] *)
-(* TODO use an attribute constraint to encode that Stage <= length name *)
-(* TODO other invariants are not encoded *)
-
-(* Wrappers for building various tuples. *)
-Open Scope Tuple_scope.
-(*Definition Build_RequestState (pac : packet) (id' : id) (stage : Stage) :=
-  < "id" :: id',
-  sQNAME :: pac!"questions"!"qname",
-  sSTAGE :: stage,
-  sQTYPE :: pac!"questions"!"qtype",
-  sQCLASS :: pac!"questions"!"qclass",
-  sPID :: pac!"id",
-  sFLAGS :: pac!"flags">%Tuple. *)
-
-Definition Build_CachePointerRow
-           (reqName : DomainName)
-           (table : CacheTable) :=
-  < sDOMAIN :: W, sCACHETABLE :: table >%Tuple.
-
-
-Definition ToSLISTRow (refRow : ReferralRow)
-           (reqId : W)
-           (refId : W)
-           (matchCount : W)
-           (queryCount : W)
-  : SLIST_ReferralRow :=
-  < sREQID :: reqId, sREFERRALID :: refId,
-  sMATCHCOUNT :: matchCount, sQUERYCOUNT :: queryCount >
-                             ++ refRow.
-
-Definition ToSLISTOrder (reqId : W)
-           (order : list refPosition) :=
-  < sREQID :: reqId, sORDER :: order >.
-
-Definition toPacket_soa (soa : FailureRow) : SOA_RDATA :=
-  prim_snd (prim_snd soa).
-
-Definition toPacket_ans (ans : AnswerRow) : resourceRecord :=
-  prim_snd (prim_snd (prim_snd ans)).
-
-(* So long strings of Ascii Bool Bool... won't show up in Set Printing All *)
-Definition Init := "Init".
-Definition MakeId := "MakeId".
-Definition AddRequest := "AddRequest".
-Definition GetRequestStage := "GetRequestStage".
-Definition UpdateRequestStage := "UpdateRequestStage".
-Definition GetServerForLongestSuffix := "GetServerForLongestSuffix".
-Definition InsertResultForDomain := "InsertResultForDomain".
-Definition DeletePendingRequestInfo := "DeletePendingRequestInfo".
-Definition DeleteCachedNameResult := "DeleteCachedNameResult".
-Definition PacketToReferralRows :="PacketToReferralRows".
-Definition InsertReferralRowsIntoCache := "InsertReferralRowsIntoCache".
-Definition ReferralRowsToSLIST := "ReferralRowsToSLIST".
-Definition GetFirstReferralAndUpdateSLIST := "GetFirstReferralAndUpdateSLIST".
-Definition SortSLIST := "SortSLIST".
-Definition UpdateCacheReferralsAndSLIST := "UpdateCacheReferralsAndSLIST".
-Definition UpdateTTLs := "UpdateTTLs".
-Definition Process := "Process".
-
-Coercion
-
-Definition default_refresh_time : W := natToWord _ 3600. (* seconds *)
-Definition default_retry_time : W := natToWord _ 600.
-Definition default_expire_time : W := natToWord _ 600.
-(* may cause stack overflow / segfault; use hours instead? *)
-Definition default_minimum_TTL : W := natToWord _ 3600.
+Definition requestTTL : timeT := 500.
+Definition serverTTL : timeT := 500.
+Definition cachedTTL : timeT := 500.
